new_proof/OperationalSemanticsProp.v
@@ -139,6 +139,23 @@ Proof.
   - right. eexists; eauto.
 Qed.
 
+(* Lemma letapp_reduction_spec_: forall n T1 e1 (v2 : value) (v : value) e, *)
+(*     tletapp v1 v2 e ↪{n} v <-> *)
+(*       (exists n' (v_x:value), n = S n' /\ *)
+(*           tletapp v1 v2 (vbvar 0) ↪{1} v_x /\ tlet () e ^t^ v_x ↪{n'} v). *)
+(* Proof. *)
+(*   split; intros. *)
+(*   - destruct n; invclear H. invclear H1. *)
+(*     + exists n. repeat split; auto; step_length_regular_solver1. invclear H. *)
+(*     destruct (letapp_reduction_spec_aux v1 v2 _ _ H1); repeat destruct_hyp_conj; subst; invclear H1. *)
+(*     + left. repeat eexists; eauto. *)
+(*     + right. repeat eexists; eauto. *)
+(*   - repeat destruct_hyp_conj; subst. *)
+(*     destruct H3; repeat destruct_hyp_conj; subst. *)
+(*     + econstructor; eauto. econstructor; eauto; lc_solver. *)
+(*     + econstructor; eauto. econstructor; eauto; lc_solver. *)
+(* Qed. *)
+
 Lemma letapp_reduction_spec: forall n (v1 v2 : value) (v : value) e,
     tletapp v1 v2 e ↪{n} v <->
       exists n', n = S n' /\ lc v1 /\ lc v2 /\ body e /\
