new_proof/RDInv2.v
@@ -1,0 +1,769 @@
+From stdpp Require Import mapset.
+From stdpp Require Import natmap.
+From stdpp Require Import fin_map_dom.
+From CT Require Import CoreLangProp.
+From CT Require Import OperationalSemanticsProp.
+From CT Require Import BasicTypingProp.
+From CT Require Import SyntaxSugar.
+From CT Require Import Refinement.
+From CT Require Import RefinementTac.
+From CT Require Import RefinementDenotation.
+From CT Require Import RefinementDenotationTac.
+From CT Require Import RefinementDenotationProp.
+From CT Require Import RDInv.
+From CT Require Import TermOrdering.
+From Coq Require Import Logic.ClassicalFacts.
+From Coq Require Import Classical.
+
+Import Atom.
+Import CoreLang.
+Import CoreLangProp.
+Import Tactics.
+Import NamelessTactics.
+Import ListCtx.
+Import OperationalSemantics.
+Import OperationalSemanticsProp.
+Import BasicTyping.
+Import SyntaxSugar.
+Import Refinement.
+Import RefinementTac.
+Import RefinementDenotation.
+Import RefinementDenotationTac.
+Import RefinementDenotationProp.
+Import NamelessTactics.
+Import TermOrdering.
+Import RDInv.
+
+Global Hint Resolve mk_eq_constant_is_not_overbasety: core.
+Global Hint Resolve mk_eq_var_is_not_overbasety: core.
+Global Hint Resolve is_arr_implies_not_overbasety: core.
+Global Hint Constructors ok_dctx: core.
+Global Hint Resolve rR_implies_no_free: core.
+Global Hint Resolve ctxrR_tlete_drop_halt_lhs: core.
+Global Hint Resolve rR_implies_reduction_no_free: core.
+Global Hint Resolve is_arr_implies_not_overbasety: core.
+Global Hint Resolve under_not_overbasety: core.
+
+Lemma has_basety_implies_constant_or_var: forall Γ (b: base_ty) (v: value),
+    Γ ⊢t v ⋮v b -> ((exists (n: constant), v = n) \/ (exists (y: atom), v = y)).
+Proof.
+  intros.
+  destruct v.
+  + left. eexists; eauto.
+  + right. eexists; eauto.
+  + invclear H.
+  + invclear H.
+  + invclear H.
+Qed.
+
+Lemma inv_basety_implies_constant_or_var: forall Γ st b n d ϕ (v: value),
+    (⅋{st}⟦[v:b|n|d|ϕ]⟧{Γ}) v -> ((exists (n: constant), v = n) \/ (exists (y: atom), v = y)).
+Proof.
+  intros. apply inv_ctxrR_regular in H; mydestr; eauto. invclear H.
+  eapply has_basety_implies_constant_or_var; eauto.
+Qed.
+
+(* Lemma state_subst_implies_rty_subst_eq2_forward_closed_rty *)
+(*     : ∀ (a v : atom) (Γ : list (atom * rty)) (L : aset) (c_x : constant) (x : atom) *)
+(*       (k : nat) (b : base_ty) (n : nat) (d : aset) (ϕ : refinement), *)
+(*   not_fv_in_refinement d ϕ -> a ∈ L -> *)
+(*   bound_in_refinement (n `min` k) (refinement_open k c_x ϕ) -> *)
+(*   closed_rty 0 L ({k ~r> v} [v:b|n|d|ϕ]) -> *)
+(*   closed_rty 0 L ({k ~r> {a := c_x }v v} [v:b|n|d|ϕ]). *)
+(* Proof. *)
+(*   intros. destruct (decide (a = v)); subst; auto. *)
+(*   assert ({v := c_x }v v = c_x) as Htmp. simpl; dec_solver2. rewrite Htmp. clear Htmp. *)
+(*   invclear H2; auto_ty_exfalso. constructor; auto. *)
+(*   invclear H3. constructor; auto. invclear H6. constructor; auto. *)
+(*   + unfold not_fv_in_refinement. intros. unfold refinement_open. *)
+(*     unfold not_fv_in_refinement in H2. unfold refinement_open in H2. *)
+(*     unfold refinement_set_open in H6. *)
+(*     apply H2 in H6. *)
+
+(*     unfold not_fv_in_refinement in H2. intros. *)
+(*     apply H2. intros. apply H7; auto. *)
+
+(*     invclear H2. constructor; auto. invclear H7. constructor; auto. *)
+(*       unfold not_fv_in_refinement. intros. apply H. intros. apply H7; auto. *)
+(*     + invclear H3. constructor; auto. *)
+(*     + simpl in H4. simpl. set_solver. *)
+
+Lemma state_subst_implies_rty_subst_eq2_forward_ok_dctx
+    : ∀ (a v : atom) (Γ : list (atom * rty)) (L : aset) (c_x : constant) (x : atom)
+      (k : nat) (b : base_ty) (n : nat) (d : aset) (ϕ : refinement),
+  not_fv_in_refinement d ϕ -> a ∈ L ->
+  bound_in_refinement (n `min` k) (refinement_open k c_x ϕ) ->
+  ok_dctx L (Γ ++ [(x, {k ~r> v} [v:b|n|d|ϕ])]) ->
+  ok_dctx L (Γ ++ [(x, {k ~r> {a := c_x }v v} [v:b|n|d|ϕ])]).
+Proof.
+  intros a v. induction Γ; intros.
+  - denotation_simp. destruct (decide (a = v)); subst; auto.
+    invclear H2; auto_ty_exfalso. constructor; auto.
+    invclear H7. constructor; auto.
+    + invclear H2. constructor; auto. invclear H7. constructor; auto.
+      unfold not_fv_in_refinement. intros. apply H. intros. apply H7; auto.
+    + invclear H3. constructor; auto.
+    + simpl in H4. simpl. set_solver.
+  - mydestr. invclear H2; auto_ty_exfalso.
+    + constructor; auto; fold (@app (atom * rty)). listctx_set_simpl.
+      eapply IHΓ; eauto. set_solver.
+    + apply ok_dctx_cons_arr; auto; fold (@app (atom * rty)). listctx_set_simpl.
+Qed.
+
+Lemma state_subst_implies_rty_subst_eq2_forward
+  : ∀ (a v : atom) (Γ : list (atom * rty)) (st : state) (c_x : constant) (τ : rty) (x : atom)
+      (k : nat) (b : base_ty) (n : nat) (d : aset) (ϕ : refinement) (e : tm),
+    ok_dctx (dom aset (<[a:=c_x]> st)) (Γ ++ [(x, {k ~r> {a := c_x }v v} [v:b|n|d|ϕ])]) ->
+    (⅋{<[a:=c_x]> st}⟦τ⟧{Γ ++ [(x, {k ~r> v} [v:b|n|d|ϕ])] }) e ->
+    (⅋{<[a:=c_x]> st}⟦τ⟧{Γ ++ [(x, {k ~r> {a := c_x }v v} [v:b|n|d|ϕ])] }) e.
+Proof.
+  intros.
+  assert (ok_dctx (dom aset (<[a:=c_x]> st)) (Γ ++ [(x, {k ~r> {a := c_x }v v} [v:b|n|d|ϕ])]) /\
+         (⅋{<[a:=c_x]> st}⟦τ⟧{Γ ++ [(x, {k ~r> v} [v:b|n|d|ϕ])] }) e). split; auto.
+  rewrite <- state_subst_implies_rty_subst_eq2 in H1; mydestr; auto.
+Qed.
+
+Lemma state_subst_implies_rty_subst_eq2_backward
+  : ∀ (a v : atom) (Γ : list (atom * rty)) (st : state) (c_x : constant) (τ : rty) (x : atom)
+      (k : nat) (b : base_ty) (n : nat) (d : aset) (ϕ : refinement) (e : tm),
+    ok_dctx (dom aset (<[a:=c_x]> st)) (Γ ++ [(x, {k ~r> v} [v:b|n|d|ϕ])]) ->
+    (⅋{<[a:=c_x]> st}⟦τ⟧{Γ ++ [(x, {k ~r> {a := c_x }v v} [v:b|n|d|ϕ])] }) e ->
+    (⅋{<[a:=c_x]> st}⟦τ⟧{Γ ++ [(x, {k ~r> v} [v:b|n|d|ϕ])] }) e.
+Proof.
+  intros.
+  assert (ok_dctx (dom aset (<[a:=c_x]> st)) (Γ ++ [(x, {k ~r> v} [v:b|n|d|ϕ])]) /\
+         (⅋{<[a:=c_x]> st}⟦τ⟧{Γ ++ [(x, {k ~r> {a := c_x }v v} [v:b|n|d|ϕ])]  }) e). split; auto.
+  rewrite state_subst_implies_rty_subst_eq2 in H1; mydestr; auto.
+Qed.
+
+Require Import Coq.Logic.FunctionalExtensionality.
+
+Lemma bstate_insert_commute: forall n1 n2 c0 c x,
+    n1 <> n2 ->
+  (<b[n2:=c0]> (<b[n1:=c]> x)) = (<b[n1:=c]> (<b[n2:=c0]> x)).
+Proof.
+  unfold bstate_insert. intros.
+  apply functional_extensionality; intros.
+  dec_solver2.
+Qed.
+
+Lemma rty_open_commute: forall n1 n2 (v1 v2: value) b d n ϕ,
+    lc v1 -> lc v2 -> n1 <> n2 ->
+    {n1 ~r> v1} ({n2 ~r> v2} [v:b|d|n|ϕ]) = {n2 ~r> v2} ({n1 ~r> v1} [v:b|d|n|ϕ]).
+Proof.
+  intros. simpl. assert ((d `min` n2) `min` n1 = (d `min` n1) `min` n2). lia. rewrite H2. clear H2.
+  assert (refinement_set_open n1 v1 (refinement_set_open n2 v2 n) = refinement_set_open n2 v2 (refinement_set_open n1 v1 n)).
+  unfold refinement_set_open.
+  destruct v1; destruct v2; auto. set_solver.
+  rewrite H2. clear H2.
+  assert (refinement_open n1 v1 (refinement_open n2 v2 ϕ) = refinement_open n2 v2 (refinement_open n1 v1 ϕ)).
+  unfold refinement_open.
+  do 3 (apply functional_extensionality; intros).
+  destruct v1; destruct v2; try destruct (x0 !! atom); try destruct (x0 !! atom0); auto;
+  try (rewrite bstate_insert_commute; auto).
+  rewrite H2; auto.
+Qed.
+
+Lemma rty_open_commute_op: forall n1 n2 (v1 v2: value) op,
+    lc v1 -> lc v2 -> n1 <> n2 ->
+    {n1 ~r> v1} ({n2 ~r> v2} (mk_op_ret op)) = {n2 ~r> v2} ({n1 ~r> v1} (mk_op_ret op)).
+Proof.
+  intros. unfold mk_op_ret. rewrite rty_open_commute; auto.
+Qed.
+
+Lemma tletbiop_aux1: forall op (x1:atom),
+    not_fv_in_refinement ({[x1]} ∪ ∅)
+    (refinement_open 0 x1 (λ (bst : bstate) (_ : state) (v : constant), eval_op op (bst 0) (bst 1) v)).
+Proof.
+  intros. unfold not_fv_in_refinement. intros. unfold refinement_open.
+  assert (m !! x1 = m' !! x1). apply H. set_solver.
+  rewrite H0.
+  destruct (m' !! x1); auto.
+Qed.
+
+Lemma tletbiop_aux2: forall op (x1:atom) (c_x:constant),
+  bound_in_refinement 0
+    (refinement_open 1 c_x
+       (refinement_open 0 x1
+          (λ (bst : bstate) (_ : state) (v : constant), eval_op op (bst 0) (bst 1) v))).
+Proof.
+  intros. unfold bound_in_refinement. intros. unfold refinement_open.
+  destruct (st !! x1); auto.
+Qed.
+
+Lemma bstate_insert_insert:
+  ∀ (n1 : nat) (c0 c : constant) (x : bstate), <b[n1:=c0]> (<b[n1:=c]> x) = <b[n1:=c0]> x.
+Proof.
+  intros. unfold bstate_insert. apply functional_extensionality; intros.
+  dec_solver2.
+Qed.
+
+Lemma subst_var_same_value: forall (x: atom) (v: value), {x := v }v x = v.
+Proof. intros. simpl. dec_solver2. Qed.
+Lemma subst_var_same_tm: forall (x: atom) (v: value), {x := v }t x = v.
+Proof. intros. simpl. dec_solver2. Qed.
+Lemma subst_var_diff_value: forall (x y: atom) (v: value), x <> y -> {x := v }v y = y.
+Proof. intros. simpl. dec_solver2. Qed.
+Lemma subst_var_diff_tm: forall (x y: atom) (v: value), x <> y -> {x := v }t y = y.
+Proof. intros. simpl. dec_solver2. Qed.
+Lemma tletbiop_aux3: forall (x1 x0: atom) (c_x: value),
+    lc c_x -> lc ({x1 := c_x }v x0).
+Proof. intros. simpl. dec_solver2. Qed.
+Lemma tletbiop_aux4: forall (x1 x0: atom) (c_x: constant),
+    lc ({x1 := c_x }v x0).
+Proof. intros. apply tletbiop_aux3. auto. Qed.
+Global Hint Resolve tletbiop_aux4: core.
+Lemma tletbiop_aux5: forall (x1: atom) (x0 c_x: constant),
+    lc ({x1 := c_x }v x0).
+Proof. intros. simpl. auto. Qed.
+Global Hint Resolve tletbiop_aux5: core.
+
+Lemma subst_over_constant: forall (x: atom) (v: value) (c_x:constant), ({x := v }v c_x) = c_x.
+Proof. intros. auto. Qed.
+
+Ltac biop_simpl:=
+  repeat
+    match goal with
+    | [H: context [{?x := ?v }v (vfvar ?x)] |- _ ] => rewrite (subst_var_same_value x v) in H
+    | [H: context [{?x := ?v }t (tvalue (vfvar ?x))] |- _ ] => rewrite (subst_var_same_tm x v) in H
+    | [|- context [{?x := ?v }v (vfvar ?x)] ] => rewrite (subst_var_same_value x v)
+    | [|- context [{?x := ?v }t (tvalue (vfvar ?x))] ] => rewrite (subst_var_same_tm x v)
+    | [H: context [{?x := ?v }v (vfvar ?y)] |- _ ] =>
+        assert (x <> y) as Htmp by auto;
+        rewrite (subst_var_diff_value x y v Htmp) in H;
+        try clear Htmp
+    | [H: context [{?x := ?v }t (tvalue (vfvar ?y))] |- _ ] =>
+        assert (x <> y) as Htmp by auto;
+        rewrite (subst_var_diff_tm x y v Htmp) in H;
+        try clear Htmp
+    | [|- context [{?x := ?v }v (vfvar ?y)] ] =>
+        assert (x <> y) as Htmp by auto;
+        rewrite (subst_var_diff_value x y v Htmp);
+        try clear Htmp
+    | [|- context [{?x := ?v }t (tvalue (vfvar ?y))] ] =>
+        assert (x <> y) as Htmp by auto;
+        rewrite (subst_var_diff_tm x y v Htmp);
+        try clear Htmp
+    | [H: context [{?x := ?v }v (vconst ?c_x) ] |- _ ] =>
+        rewrite (subst_over_constant x v c_x) in H
+    | [|- context [{?x := ?v }v (vconst ?c_x) ] ] =>
+        rewrite (subst_over_constant x v c_x)
+    end.
+
+Lemma state_subst_implies_rty_subst_eq2_forward2
+  : ∀ (a: atom) (Γ : list (atom * rty)) (st : state) (c_x : constant) (τ : rty) (x : atom)
+      (k : nat) (b : base_ty) (n : nat) (d : aset) (ϕ : refinement) (e : tm),
+    not_fv_in_refinement d ϕ -> bound_in_refinement (n `min` k) (refinement_open k c_x ϕ) ->
+    (⅋{<[a:=c_x]> st}⟦τ⟧{Γ ++ [(x, {k ~r> a} [v:b|n|d|ϕ])] }) e ->
+    (⅋{<[a:=c_x]> st}⟦τ⟧{Γ ++ [(x, {k ~r> c_x} [v:b|n|d|ϕ])] }) e.
+Proof.
+  intros. apply state_subst_implies_rty_subst_eq2_forward in H1; biop_simpl; auto.
+  apply inv_ctxrR_regular in H1; mydestr.
+  apply state_subst_implies_rty_subst_eq2_forward_ok_dctx with (a:=a) (c_x:=c_x) in H2;  biop_simpl; eauto.
+  rewrite dom_insert_simp. set_solver.
+Qed.
+
+Lemma bound_in_refinement_open_minus1: forall n (v1: value) ϕ,
+    ((exists (n: constant), v1 = n) \/ (exists (y: atom), v1 = y)) ->
+    bound_in_refinement (S n) ϕ -> bound_in_refinement n (refinement_open n v1 ϕ).
+Proof.
+  unfold bound_in_refinement; unfold refinement_open. intros. destruct H; mydestr; subst.
+  - apply H0. apply bst_eq_insert_S; auto.
+  - destruct (st !! x).
+    + apply H0. apply bst_eq_insert_S; auto.
+    + apply H0. apply bst_eq_insert_S; auto.
+Qed.
+
+Lemma state_subst_implies_rty_subst_eq2_forward_closed_rty
+  : ∀ (a v: atom) (L d: aset) (c_x : constant)
+      (k : nat) (b : base_ty) (m n : nat) (ϕ : refinement),
+    not_fv_in_refinement d ϕ -> bound_in_refinement (n `min` k) (refinement_open k c_x ϕ) ->
+    closed_rty m L ({k ~r> v} [v:b|n|d|ϕ]) ->
+    closed_rty m L ({k ~r> {a := c_x }v v} [v:b|n|d|ϕ]).
+Proof.
+  intros. destruct (decide (a = v)); subst; auto; biop_simpl; auto.
+  invclear H1. constructor; auto.
+  - constructor; auto. constructor; auto.
+    unfold not_fv_in_refinement. unfold refinement_open. intros.
+    apply H; auto.
+  - invclear H3. constructor; auto.
+  - simpl in H4. simpl. fast_set_solver.
+Qed.
+
+Lemma state_subst_implies_rty_subst_eq2_rR
+  : ∀ (a v: atom) st bst (c_x : constant)
+      (k : nat) (b : base_ty) m (n : nat) (d : aset) (ϕ : refinement) e,
+    (closed_rty m (dom aset (<[a:=c_x]> st)) ({k ~r> {a := c_x }v v} [v:b|n|d|ϕ]) /\
+       {m;bst;(<[a:=c_x]> st)}⟦ {k ~r> v} [v:b|n|d|ϕ]⟧ e) <->
+      (closed_rty m (dom aset (<[a:=c_x]> st)) ({k ~r> v} [v:b|n|d|ϕ]) /\
+         {m;bst;(<[a:=c_x]> st)}⟦ {k ~r> {a := c_x }v v} [v:b|n|d|ϕ] ⟧ e).
+Proof.
+  split; intros; mydestr.
+  - split; auto. refinement_solver.
+    destruct (decide (a = v)); subst; auto; biop_simpl; auto.
+    invclear H0; mydestr. constructor; auto. split; auto.
+    intros. apply H2; auto. unfold refinement_open. my_simplify_map_eq3.
+  - split; auto. refinement_solver.
+    destruct (decide (a = v)); subst; auto; biop_simpl; auto.
+    invclear H0; mydestr. constructor; auto. split; auto.
+    intros. apply H2; auto. unfold refinement_open in H4.
+    my_simplify_map_eq3.
+Qed.
+
+Lemma state_subst_implies_rty_subst_eq2_rR_forward
+  : ∀ (a v: atom) st bst (c_x : constant)
+      (k : nat) (b : base_ty) m (n : nat) (d : aset) (ϕ : refinement) e,
+    closed_rty m (dom aset (<[a:=c_x]> st)) ({k ~r> {a := c_x }v v} [v:b|n|d|ϕ]) ->
+    {m;bst;(<[a:=c_x]> st)}⟦ {k ~r> v} [v:b|n|d|ϕ]⟧ e ->
+    {m;bst;(<[a:=c_x]> st)}⟦ {k ~r> {a := c_x }v v} [v:b|n|d|ϕ] ⟧ e.
+Proof.
+  intros.
+  assert (closed_rty m (dom aset (<[a:=c_x]> st)) ({k ~r> {a := c_x }v v} [v:b|n|d|ϕ]) /\
+         {m;bst;(<[a:=c_x]> st)}⟦ {k ~r> v} [v:b|n|d|ϕ]⟧ e); auto.
+  rewrite state_subst_implies_rty_subst_eq2_rR in H1; mydestr; auto.
+Qed.
+
+Lemma state_subst_implies_rty_subst_eq2_rR_backward
+  : ∀ (a v: atom) st bst (c_x : constant)
+      (k : nat) (b : base_ty) m (n : nat) (d : aset) (ϕ : refinement) e,
+    closed_rty m (dom aset (<[a:=c_x]> st)) ({k ~r> v} [v:b|n|d|ϕ]) ->
+    {m;bst;(<[a:=c_x]> st)}⟦ {k ~r> {a := c_x }v v} [v:b|n|d|ϕ] ⟧ e ->
+    {m;bst;(<[a:=c_x]> st)}⟦ {k ~r> v} [v:b|n|d|ϕ]⟧ e.
+Proof.
+  intros.
+  assert (closed_rty m (dom aset (<[a:=c_x]> st)) ({k ~r> v} [v:b|n|d|ϕ]) /\
+         {m;bst;(<[a:=c_x]> st)}⟦ {k ~r> {a := c_x }v v} [v:b|n|d|ϕ] ⟧ e); auto.
+  rewrite <- state_subst_implies_rty_subst_eq2_rR in H1; mydestr; auto.
+Qed.
+
+Lemma state_insert_include_a: forall (a: atom) (st: state) (c_x: constant),
+    a ∈ dom aset (<[a:=c_x]> st).
+Proof.
+  intros. rewrite dom_insert_simp; auto. set_solver.
+Qed.
+
+Global Hint Resolve state_insert_include_a: core.
+
+Lemma state_subst_implies_rty_subst_eq2_forward_wf_ctxrR
+    : ∀ (a v : atom) (Γ : list (atom * rty)) st (c_x : constant) (x : atom)
+      (k : nat) (b : base_ty) (n : nat) (d : aset) (ϕ : refinement),
+  not_fv_in_refinement d ϕ -> a ∉ (stale st ∪ stale Γ ∪ {[x]}) ->
+  bound_in_refinement (n `min` k) (refinement_open k c_x ϕ) ->
+  wf_ctxrR (<[a:=c_x]> st) (Γ ++ [(x, {k ~r> v} [v:b|n|d|ϕ])]) ->
+  wf_ctxrR (<[a:=c_x]> st) (Γ ++ [(x, {k ~r> {a := c_x }v v} [v:b|n|d|ϕ])]).
+Proof.
+  intros a v. induction Γ; intros.
+  - listctx_set_simpl.
+    assert (ok_dctx (dom aset (<[a:=c_x]> st)) ([] ++ [(x, {k ~r> v} [v:b|n|d|ϕ])])).
+    { apply wf_ctxrR_regular1 in H2; auto. }
+    constructor; auto.
+    + eapply state_subst_implies_rty_subst_eq2_forward_ok_dctx in H3; eauto.
+    + invclear H2; auto; try auto_ty_exfalso. intros. apply H12.
+      assert ({0;b∅;<[a:=c_x]> st}⟦ {k ~r> {a := c_x }v v} [v:b|n|d|ϕ] ⟧ e_wf); auto.
+      apply state_subst_implies_rty_subst_eq2_rR_backward in H4; auto.
+      refinement_solver.
+    + invclear H2; auto; try auto_ty_exfalso. mydestr. exists x0. split; eauto.
+       assert ({0;b∅;<[a:=c_x]> st}⟦ {k ~r> v} [v:b|n|d|ϕ] ⟧ x0); auto.
+       apply state_subst_implies_rty_subst_eq2_rR_forward in H5; auto.
+       apply state_subst_implies_rty_subst_eq2_forward_closed_rty; auto.
+       refinement_solver.
+  - RD_simp2.
+    + constructor; auto.
+      { rewrite app_comm_cons.
+        apply state_subst_implies_rty_subst_eq2_forward_ok_dctx; auto. }
+      intros. setoid_rewrite insert_commute; try fast_set_solver.
+      apply IHΓ; auto. setoid_rewrite dom_insert_simp; auto. set_solver.
+      setoid_rewrite insert_commute; try fast_set_solver.
+    + mydestr. constructor; auto.
+      { rewrite app_comm_cons.
+        apply state_subst_implies_rty_subst_eq2_forward_ok_dctx; auto. }
+      exists x0. split; auto. intros. eapply H3 in H4; eauto.
+      assert (exists (c: constant), v_x = c). dsimp1; eauto. mydestr; subst.
+      setoid_rewrite insert_commute; try fast_set_solver.
+      apply IHΓ; auto. setoid_rewrite dom_insert_simp; auto. set_solver.
+      setoid_rewrite insert_commute; try fast_set_solver.
+    + constructor; auto.
+      { rewrite app_comm_cons.
+        apply state_subst_implies_rty_subst_eq2_forward_ok_dctx; auto. }
+      apply IHΓ; auto. set_solver.
+Qed.
+
+Lemma state_subst_implies_rty_subst_eq2_forwardc_wf_ctxrR
+    : ∀ (a : atom) (Γ : list (atom * rty)) st (c_x : constant) (x : atom)
+      (k : nat) (b : base_ty) (n : nat) (d : aset) (ϕ : refinement),
+  not_fv_in_refinement d ϕ -> a ∉ (stale st ∪ stale Γ ∪ {[x]}) ->
+  bound_in_refinement (n `min` k) (refinement_open k c_x ϕ) ->
+  wf_ctxrR (<[a:=c_x]> st) (Γ ++ [(x, {k ~r> a} [v:b|n|d|ϕ])]) ->
+  wf_ctxrR (<[a:=c_x]> st) (Γ ++ [(x, {k ~r> c_x} [v:b|n|d|ϕ])]).
+Proof.
+  intros.
+  apply state_subst_implies_rty_subst_eq2_forward_wf_ctxrR in H2; biop_simpl; auto.
+Qed.
+
+Lemma state_subst_implies_rty_subst_eq2_backward_wf_ctxrR
+    : ∀ (a v : atom) (Γ : list (atom * rty)) st (c_x : constant) (x : atom)
+      (k : nat) (b : base_ty) (n : nat) (d : aset) (ϕ : refinement),
+  a ∉ (stale st ∪ stale Γ ∪ {[x]}) ->
+  ok_dctx (dom aset (<[a:=c_x]> st)) (Γ ++ [(x, {k ~r> v} [v:b|n|d|ϕ])]) ->
+  wf_ctxrR (<[a:=c_x]> st) (Γ ++ [(x, {k ~r> {a := c_x }v v} [v:b|n|d|ϕ])]) ->
+  wf_ctxrR (<[a:=c_x]> st) (Γ ++ [(x, {k ~r> v} [v:b|n|d|ϕ])]).
+Proof.
+  intros a v. induction Γ; intros.
+  - listctx_set_simpl.
+    constructor; auto.
+    + invclear H1; auto; try auto_ty_exfalso. intros. apply H10.
+      assert ({0;b∅;<[a:=c_x]> st}⟦ {k ~r> {a := c_x }v v} [v:b|n|d|ϕ] ⟧ e_wf); auto.
+      apply state_subst_implies_rty_subst_eq2_rR_forward in H1; auto.
+      refinement_solver.
+    + invclear H1; auto; try auto_ty_exfalso. mydestr. exists x0. split; eauto.
+       assert ({0;b∅;<[a:=c_x]> st}⟦ {k ~r> {a := c_x }v v} [v:b|n|d|ϕ] ⟧ x0); auto.
+       apply state_subst_implies_rty_subst_eq2_rR_backward in H3; auto.
+       refinement_solver.
+  - RD_simp2; invclear H0; try auto_ty_exfalso.
+    + constructor; auto.
+      intros. setoid_rewrite insert_commute; try fast_set_solver.
+      apply IHΓ; auto. setoid_rewrite dom_insert_simp; auto. set_solver.
+      setoid_rewrite insert_commute; try fast_set_solver. setoid_rewrite dom_insert_simp; auto.
+      setoid_rewrite insert_commute; try fast_set_solver.
+    + mydestr. constructor; auto.
+      exists x0. split; auto. intros. eapply H1 in H2; eauto.
+      assert (exists (c: constant), v_x = c). dsimp1; eauto. mydestr; subst.
+      setoid_rewrite insert_commute; try fast_set_solver.
+      apply IHΓ; auto. setoid_rewrite dom_insert_simp; auto. set_solver.
+      setoid_rewrite insert_commute; try fast_set_solver. setoid_rewrite dom_insert_simp; auto.
+      setoid_rewrite insert_commute; try fast_set_solver.
+    + constructor; auto.
+      apply IHΓ; auto. set_solver.
+Qed.
+
+Lemma tletbiop_aux6: forall op (v1 v2: value),
+    ((exists (n: constant), v1 = n) \/ (exists (y: atom), v1 = y)) ->
+    ((exists (n: constant), v2 = n) \/ (exists (y: atom), v2 = y)) ->
+    bound_in_refinement 0
+      (refinement_open 1 v1
+         (refinement_open 0 v2
+            (λ (bst : bstate) (_ : state) (v : constant), eval_op op (bst 0) (bst 1) v))).
+Proof.
+  unfold bound_in_refinement; unfold refinement_open. intros.
+  destruct H; destruct H0; mydestr;
+    try (try destruct (st !! x); auto; try destruct (st !! x0); subst; auto);
+    try (destruct (st !! x); auto);
+    try (destruct (st !! x0); auto).
+Qed.
+
+Lemma tletbiop_aux7: forall op (v1 v2: value),
+    ((exists (n: constant), v1 = n) \/ (exists (y: atom), v1 = y)) ->
+    ((exists (n: constant), v2 = n) \/ (exists (y: atom), v2 = y)) ->
+    bound_in_refinement 0
+      (refinement_open 0 v1
+         (refinement_open 1 v2
+            (λ (bst : bstate) (_ : state) (v : constant), eval_op op (bst 0) (bst 1) v))).
+Proof.
+  unfold bound_in_refinement; unfold refinement_open. intros.
+  destruct H; destruct H0; mydestr;
+    try (try destruct (st !! x); auto; try destruct (st !! x0); subst; auto);
+    try (destruct (st !! x); auto);
+    try (destruct (st !! x0); auto).
+Qed.
+
+Lemma tletbiop_aux8: forall (d: aset), (d ∪ ∅) = d.
+Proof.
+  intros. set_solver. Qed.
+
+Lemma not_fv_in_refinement_aux: forall op (v: value) (n: nat),
+    n ≤ 1 -> ((exists (n: constant), v = n) \/ (exists (y: atom), v = y)) ->
+    not_fv_in_refinement (fv_value v)
+      (refinement_open n v
+         (λ (bst : bstate) (_ : state) (v : constant), eval_op op (bst 0) (bst 1) v)).
+Proof.
+  unfold not_fv_in_refinement; unfold refinement_open. intros.
+  destruct H0; mydestr; subst; auto.
+  assert (m !! x = m' !! x). apply H1; fast_set_solver. rewrite H0.
+  destruct (m'!!x); auto.
+Qed.
+
+Lemma mk_op_ret_wf_ctxrR
+    : ∀ st op (a : atom) (v1 v2: value) (Γ : list (atom * rty)) (c_x : constant) (x: atom),
+    ((exists (n: constant), v1 = n) \/ (exists (y: atom), v1 = y)) ->
+    ((exists (n: constant), v2 = n) \/ (exists (y: atom), v2 = y)) ->
+    a ∉ stale st ∪ stale Γ ∪ {[x]} ->
+    (ok_dctx (dom aset (<[a:=c_x]> st)) (Γ ++ [(x, {1 ~r> v2} (mk_op_ret op ^r^ v1))]) /\
+       (wf_ctxrR (<[a:=c_x]> st)
+          (Γ ++ [(x, {1 ~r> ({a := c_x }v v2)} (mk_op_ret op ^r^ ({a := c_x }v v1)))]))
+    ) <-> (wf_ctxrR (<[a:=c_x]> st) (Γ ++ [(x, {1 ~r> v2} (mk_op_ret op ^r^ v1))])).
+Proof.
+  split; intros; mydestr; subst.
+  - destruct H; destruct H0; mydestr; subst; auto.
+    + destruct (decide (a = x0)); auto; subst; biop_simpl; auto.
+      apply state_subst_implies_rty_subst_eq2_backward_wf_ctxrR; biop_simpl; auto.
+    + destruct (decide (a = x1)); auto; subst; biop_simpl; auto.
+      rewrite rty_open_commute_op; auto.
+      rewrite rty_open_commute_op in H3; auto.
+      rewrite rty_open_commute_op in H2; auto.
+      apply state_subst_implies_rty_subst_eq2_backward_wf_ctxrR; biop_simpl; auto.
+    + destruct (decide (a = x0)); auto; subst; auto.
+      { biop_simpl.
+        destruct (decide (x0 = x1)); auto; subst.
+        - biop_simpl.
+          assert (ok_dctx (dom aset (<[x1:=c_x]> st)) (Γ ++ [(x, {1 ~r> c_x} (mk_op_ret op ^r^ x1))])).
+          { apply state_subst_implies_rty_subst_eq2_forward_ok_dctx with (a:=x1) (c_x :=c_x) in H2; eauto. biop_simpl; auto.
+          unfold refinement_set_open. apply tletbiop_aux1; auto.
+          assert ((2 `min` 0) `min` 1 = 0) by lia. setoid_rewrite H. clear H.
+          apply tletbiop_aux2. }
+          assert (wf_ctxrR (<[x1:=c_x]> st) (Γ ++ [(x, {1 ~r> c_x} (mk_op_ret op ^r^ x1))])).
+          { rewrite rty_open_commute_op; auto.
+            rewrite rty_open_commute_op in H3; auto.
+            rewrite rty_open_commute_op in H; auto.
+            apply state_subst_implies_rty_subst_eq2_backward_wf_ctxrR; biop_simpl; auto. }
+          apply state_subst_implies_rty_subst_eq2_backward_wf_ctxrR; biop_simpl; auto.
+        - apply state_subst_implies_rty_subst_eq2_backward_wf_ctxrR; biop_simpl; auto.
+      }
+      { rewrite rty_open_commute_op in H2; auto.
+        rewrite rty_open_commute_op in H3; auto.
+        rewrite rty_open_commute_op; auto.
+        apply state_subst_implies_rty_subst_eq2_backward_wf_ctxrR; biop_simpl; auto.
+ }
+ - split. apply wf_ctxrR_regular1 in H2; mydestr; auto.
+    destruct H; destruct H0; mydestr; subst; auto.
+    + destruct (decide (a = x0)); auto; subst; biop_simpl; auto.
+      apply state_subst_implies_rty_subst_eq2_forwardc_wf_ctxrR; biop_simpl; auto.
+      pose (not_fv_in_refinement_aux op x1 0) as Hn; apply Hn; try lia; eauto.
+      apply tletbiop_aux6; eauto.
+    + destruct (decide (a = x1)); auto; subst; biop_simpl; auto.
+      rewrite rty_open_commute_op; auto.
+      rewrite rty_open_commute_op in H2; auto.
+      apply state_subst_implies_rty_subst_eq2_forwardc_wf_ctxrR; biop_simpl; auto.
+      pose (not_fv_in_refinement_aux op x0 1) as Hn; apply Hn; try lia; eauto.
+      apply tletbiop_aux7; eauto.
+    + destruct (decide (a = x0)); auto; subst; auto; biop_simpl.
+      { destruct (decide (x0 = x1)); auto; subst; biop_simpl.
+        - assert (wf_ctxrR (<[x1:=c_x]> st) (Γ ++ [(x, {1 ~r> x1} (mk_op_ret op ^r^ c_x))] )).
+          rewrite rty_open_commute_op; auto.
+          rewrite rty_open_commute_op in H2; auto.
+          apply state_subst_implies_rty_subst_eq2_forwardc_wf_ctxrR; biop_simpl; auto.
+          pose (not_fv_in_refinement_aux op x1 1) as Hn; simpl; rewrite tletbiop_aux8; apply Hn; try lia; eauto.
+          simpl. apply tletbiop_aux7; eauto.
+          apply state_subst_implies_rty_subst_eq2_forwardc_wf_ctxrR; biop_simpl; auto.
+          pose (not_fv_in_refinement_aux op c_x 0) as Hn; simpl; try rewrite tletbiop_aux8; apply Hn; try lia; eauto.
+          simpl. apply tletbiop_aux6; eauto.
+        - apply state_subst_implies_rty_subst_eq2_forwardc_wf_ctxrR; biop_simpl; auto.
+          pose (not_fv_in_refinement_aux op x1 0) as Hn; simpl; try rewrite tletbiop_aux8; apply Hn; try lia; eauto.
+          simpl. apply tletbiop_aux6; eauto.
+      }
+      { destruct (decide (a = x1)); auto; subst; biop_simpl; auto.
+        rewrite rty_open_commute_op; auto.
+        rewrite rty_open_commute_op in H2; auto.
+        apply state_subst_implies_rty_subst_eq2_forwardc_wf_ctxrR; biop_simpl; auto.
+        pose (not_fv_in_refinement_aux op x0 1) as Hn; simpl; try rewrite tletbiop_aux8; apply Hn; try lia; eauto.
+        simpl. apply tletbiop_aux7; eauto.
+      }
+Qed.
+
+Lemma mk_op_ret_ok_dctx
+    : ∀ st op (a : atom) (v1 v2: value) (Γ : list (atom * rty)) (c_x : constant) (x : atom) e τ,
+    ((exists (n: constant), v1 = n) \/ (exists (y: atom), v1 = y)) ->
+    ((exists (n: constant), v2 = n) \/ (exists (y: atom), v2 = y)) ->
+    (ok_dctx (dom aset (<[a:=c_x]> st)) (Γ ++ [(x, {1 ~r> v2} (mk_op_ret op ^r^ v1))]) /\
+    (⅋{<[a:=c_x]> st}⟦τ⟧{Γ ++ [(x, {1 ~r> ({a := c_x }v v2)} (mk_op_ret op ^r^ ({a := c_x }v v1)))] } e)) <->
+       (⅋{<[a:=c_x]> st}⟦τ⟧{Γ ++ [(x, {1 ~r> v2} (mk_op_ret op ^r^ v1))] }) e.
+Proof.
+  split; intros; mydestr; subst.
+  - destruct H; destruct H0; mydestr; subst; auto.
+    + destruct (decide (a = x0)); auto; subst; biop_simpl; auto.
+      apply state_subst_implies_rty_subst_eq2_backward; biop_simpl; auto.
+    + destruct (decide (a = x1)); auto; subst; biop_simpl; auto.
+      rewrite rty_open_commute_op; auto.
+      rewrite rty_open_commute_op in H1; auto.
+      rewrite rty_open_commute_op in H2; auto.
+      apply state_subst_implies_rty_subst_eq2_backward; biop_simpl; auto.
+    + destruct (decide (a = x0)); auto; subst; auto.
+      { biop_simpl.
+        destruct (decide (x0 = x1)); auto; subst.
+        - biop_simpl.
+          assert (ok_dctx (dom aset (<[x1:=c_x]> st)) (Γ ++ [(x, {1 ~r> c_x} (mk_op_ret op ^r^ x1))])).
+          { apply state_subst_implies_rty_subst_eq2_forward_ok_dctx with (a:=x1) (c_x :=c_x) in H1; eauto. biop_simpl; auto.
+          unfold refinement_set_open. apply tletbiop_aux1; auto.
+          assert ((2 `min` 0) `min` 1 = 0) by lia. setoid_rewrite H. clear H.
+          apply tletbiop_aux2. }
+          assert ((⅋{<[x1:=c_x]> st}⟦τ⟧{Γ ++ [(x, {1 ~r> c_x} (mk_op_ret op ^r^ x1))] }) e).
+          { rewrite rty_open_commute_op; auto.
+            rewrite rty_open_commute_op in H; auto.
+            rewrite rty_open_commute_op in H2; auto.
+            apply state_subst_implies_rty_subst_eq2_backward; biop_simpl; auto. }
+          apply state_subst_implies_rty_subst_eq2_backward; biop_simpl; auto.
+        - apply state_subst_implies_rty_subst_eq2_backward; biop_simpl; auto.
+      }
+      { rewrite rty_open_commute_op in H1; auto.
+        rewrite rty_open_commute_op in H2; auto.
+        rewrite rty_open_commute_op; auto.
+        apply state_subst_implies_rty_subst_eq2_backward; biop_simpl; auto. }
+  - split. try (apply inv_ctxrR_regular in H1; mydestr; auto).
+    destruct H; destruct H0; mydestr; subst; auto.
+    + destruct (decide (a = x0)); auto; subst; biop_simpl; auto.
+      apply state_subst_implies_rty_subst_eq2_forward2; biop_simpl; auto.
+      pose (not_fv_in_refinement_aux op x1 0) as Hn; apply Hn; try lia; eauto.
+      apply tletbiop_aux6; eauto.
+    + destruct (decide (a = x1)); auto; subst; biop_simpl; auto.
+      rewrite rty_open_commute_op; auto.
+      rewrite rty_open_commute_op in H1; auto.
+      apply state_subst_implies_rty_subst_eq2_forward2; biop_simpl; auto.
+      pose (not_fv_in_refinement_aux op x0 1) as Hn; apply Hn; try lia; eauto.
+      apply tletbiop_aux7; eauto.
+    + destruct (decide (a = x0)); auto; subst; auto; biop_simpl.
+      { destruct (decide (x0 = x1)); auto; subst; biop_simpl.
+        - assert ((⅋{<[x1:=c_x]> st}⟦τ⟧{Γ ++ [(x, {1 ~r> x1} (mk_op_ret op ^r^ c_x))] }) e).
+          rewrite rty_open_commute_op; auto.
+          rewrite rty_open_commute_op in H1; auto.
+          apply state_subst_implies_rty_subst_eq2_forward2; biop_simpl; auto.
+          pose (not_fv_in_refinement_aux op x1 1) as Hn; simpl; rewrite tletbiop_aux8; apply Hn; try lia; eauto.
+          simpl. apply tletbiop_aux7; eauto.
+          apply state_subst_implies_rty_subst_eq2_forward2; biop_simpl; auto.
+          pose (not_fv_in_refinement_aux op c_x 0) as Hn; simpl; try rewrite tletbiop_aux8; apply Hn; try lia; eauto.
+          simpl. apply tletbiop_aux6; eauto.
+        - apply state_subst_implies_rty_subst_eq2_forward2; biop_simpl; auto.
+          pose (not_fv_in_refinement_aux op x1 0) as Hn; simpl; try rewrite tletbiop_aux8; apply Hn; try lia; eauto.
+          simpl. apply tletbiop_aux6; eauto.
+      }
+      { destruct (decide (a = x1)); auto; subst; biop_simpl; auto.
+        rewrite rty_open_commute_op; auto.
+        rewrite rty_open_commute_op in H1; auto.
+        apply state_subst_implies_rty_subst_eq2_forward2; biop_simpl; auto.
+        pose (not_fv_in_refinement_aux op x0 1) as Hn; simpl; try rewrite tletbiop_aux8; apply Hn; try lia; eauto.
+        simpl. apply tletbiop_aux7; eauto.
+      }
+Qed.
+
+Lemma letebiop_aux9: forall op r, is_arr r -> ~ ⌊r⌋ = fst_ty_of_op op.
+Proof.
+  intros. destruct r; destruct op; simpl; invclear H; try (intro H; invclear H).
+Qed.
+
+Lemma inv_rRctx_tletbiop: forall Γ st (τ: rty) x op n1 d1 ϕ1 n2 d2 ϕ2 (v1 v2: value) e,
+    x ∉ fv_tm e -> x ∉ rty_fv τ -> not_overbasety τ ->
+    wf_ctxrR st (Γ ++ [(x, {1 ~r> v2} (mk_op_ret op ^r^ v1))]) ->
+    (⅋{st}⟦[v:fst_ty_of_op op|n1|d1|ϕ1]⟧{Γ}) v1 ->
+    (⅋{st}⟦[v:snd_ty_of_op op|n2|d2|ϕ2]⟧{Γ}) v2 ->
+    (⅋{st}⟦τ⟧{Γ ++ [(x, {1 ~r> v2} (mk_op_ret op ^r^ v1))] }) (e ^t^ x) ->
+    ⅋{st}⟦τ⟧{Γ ++ [(x, {1 ~r> v2} (mk_op_ret op ^r^ v1))] } (tletbiop op v1 v2 e).
+Proof.
+  induction Γ; intros; RD_simp2.
+  - mydestr. inv_rd_simpl1. constructor; auto.
+    + denotation_simp. assert ([] ⊢t tletbiop op v1 v2 e ⋮t ⌊τ⌋). eapply tletbiop_typable; refinement_solver.
+      basic_typing_solver.
+    + assert ((exists (m1: nat), v1 = m1)) by (eapply fst_ty_of_op_implies_nat; eauto). mydestr; subst. rename x2 into v1.
+      assert ((exists (m2: nat), v2 = m2)) by (eapply snd_ty_of_op_implies_nat; eauto). mydestr; subst. rename x2 into v2.
+      exists (eval_op_under_bound_tm op v1 v2). split. apply rR_eval_op_under_bound_tm.
+      intros. assert (x1 ↪* v_x) as Hz by (eapply rR_eval_op_under_bound_tm_min; eauto).
+      auto_under v_x. RD_simp2. simpl.
+      rewrite subst_fresh_tm; auto. rewrite open_subst_same_tm in H10; auto.
+      eapply termR_perserve_rR; refinement_solver.
+      eapply letapp_eval_op_under_bound_tm_termR; eauto; refinement_solver.
+  - constructor; auto. denotation_simp. apply tletbiop_typable_ctx_dummy_cons; auto.
+    intros. auto_under c_x. invclear H11; auto_ty_exfalso.
+    assert ((exists (n: constant), v1 = n) \/ (exists (y: atom), v1 = y)).
+    { invclear H20. eapply has_basety_implies_constant_or_var; eauto. }
+    assert ((exists (n: constant), v2 = n) \/ (exists (y: atom), v2 = y)).
+    { invclear H23. eapply has_basety_implies_constant_or_var; eauto. }
+    rewrite <- mk_op_ret_ok_dctx; auto. split; auto. rewrite dom_insert_simp; auto.
+    assert (a <> x) by (rewrite ctxdom_app_union in H16; inv_rd_simpl1).
+    eapply IHΓ; eauto; fold value_subst; fold tm_subst.
+    + pose (fv_of_subst_tm a c_x e). set_solver.
+    + assert (wf_ctxrR (<[a:=c_x]> st)
+                (Γ ++ [(x, {1 ~r> v2} (mk_op_ret op ^r^ v1))])); auto.
+      rewrite <- mk_op_ret_wf_ctxrR in H10; mydestr; auto.
+      inv_rd_simpl1.
+    + assert ((⅋{<[a:=c_x]> st}⟦τ⟧{Γ ++
+                       [(x, {1 ~r> v2} (mk_op_ret op ^r^ v1))] }) ({a := c_x }t (e ^t^ x))
+           ); auto.
+      rewrite subst_open_tm in H10; auto.
+      assert ({a := c_x}v x = x). { simpl. dec_solver2. }
+      rewrite H11 in H10.
+      rewrite <- mk_op_ret_ok_dctx in H10; mydestr; auto.
+  - constructor; auto. denotation_simp. apply tletbiop_typable_ctx_dummy_cons; auto.
+    mydestr. auto_meet_exists Hmeet. auto_meet_reduce. auto_under v_x.
+    assert ((exists (n: constant), v1 = n) \/ (exists (y: atom), v1 = y)).
+    { invclear H20. eapply has_basety_implies_constant_or_var; eauto. }
+    assert ((exists (n: constant), v2 = n) \/ (exists (y: atom), v2 = y)).
+    { invclear H23. eapply has_basety_implies_constant_or_var; eauto. }
+    assert (exists (c: constant), v_x = c). dsimp1; eauto. mydestr; subst.
+    assert (({a↦x4}) st = <[a:=x4]> st) as Htz; auto. rewrite Htz.
+    rewrite <- mk_op_ret_ok_dctx; auto. split; auto.
+    { apply inv_ctxrR_regular in H12; mydestr; auto. }
+    assert (a <> x). { apply ok_dctx_regular in H11; mydestr. basic_typing_solver. }
+    eapply IHΓ; eauto; fold value_subst; fold tm_subst.
+    + rewrite fv_of_subst_tm_closed; refinement_solver.
+    + eapply H3 in H2; eauto.
+      assert (wf_ctxrR (<[a:=x4]> st)
+                (Γ ++ [(x, {1 ~r> v2} (mk_op_ret op ^r^ v1))])); auto.
+      rewrite <- mk_op_ret_wf_ctxrR in H28; mydestr; auto.
+      apply ok_dctx_regular in H11; mydestr. simpl in H29. listctx_set_simpl.
+      set_solver.
+    + assert ((⅋{<[a:=x4]> st}⟦τ⟧{Γ ++
+                       [(x, {1 ~r> v2} (mk_op_ret op ^r^ v1))] }) ({a := x4 }t (e ^t^ x))
+           ); auto.
+      rewrite subst_open_tm in H28; auto.
+      assert ({a := x4}v x = x). { simpl. dec_solver2. }
+      rewrite H29 in H28.
+      rewrite <- mk_op_ret_ok_dctx in H28; mydestr; auto.
+  - constructor; auto. denotation_simp. apply tletbiop_typable_ctx_dummy_cons; auto.
+    intros. auto_under v_x.
+    assert ((exists (n: constant), v1 = n) \/ (exists (y: atom), v1 = y)).
+    { invclear H23. eapply has_basety_implies_constant_or_var; eauto. }
+    assert ((exists (n: constant), v2 = n) \/ (exists (y: atom), v2 = y)).
+    { invclear H19. eapply has_basety_implies_constant_or_var; eauto. }
+    assert ({a := v_x }t tletbiop op v1 v2 e =
+           tletbiop op ({a := v_x }v v1) ({a := v_x }v v2) ({a := v_x }t e)) as Htz; auto.
+    rewrite Htz.
+    assert ({a := v_x }v v1 = v1).
+    { destruct H4; mydestr; subst; auto. simpl. dec_solver2; subst.
+      invclear H23. invclear H22. simpl in H26. rewrite decide_True in H26. invclear H26.
+      apply letebiop_aux9 with (op:=op) in H6. exfalso. apply H6; auto. reflexivity.
+    }
+    assert ({a := v_x }v v2 = v2).
+    { destruct H5; mydestr; subst; auto. simpl. dec_solver2; subst.
+      invclear H19. invclear H26. simpl in H27. rewrite decide_True in H27. invclear H27.
+      apply letebiop_aux9 with (op:=op) in H6. exfalso. apply H6; auto. reflexivity.
+    }
+    rewrite H17. rewrite H22.
+    assert ({a := v_x }t v1 = v1) by (simpl; rewrite H17; auto).
+    assert ({a := v_x }t v2 = v2) by (simpl; rewrite H22; auto).
+    rewrite H26 in H24.
+    rewrite H27 in H20.
+    eapply IHΓ; eauto; fold tm_subst.
+    + rewrite fv_of_subst_tm_closed; refinement_solver.
+    + rewrite <- subst_open_var_tm; auto. denotation_simp. basic_typing_solver. refinement_solver.
+Qed.
+
+(* Lemma inv_rRctx_tletbiop: forall Γ st (τ: rty) x op n1 d1 ϕ1 n2 d2 ϕ2 (v1 v2: nat) e, *)
+(*     x ∉ fv_tm e -> x ∉ rty_fv τ -> not_overbasety τ -> *)
+(*     wf_ctxrR st (Γ ++ [(x, {1 ~r> v2} (mk_op_ret op ^r^ v1))]) -> *)
+(*     (⅋{st}⟦[v:fst_ty_of_op op|n1|d1|ϕ1]⟧{Γ}) v1 -> *)
+(*     (⅋{st}⟦[v:fst_ty_of_op op|n2|d2|ϕ2]⟧{Γ}) v2 -> *)
+(*     (⅋{st}⟦τ⟧{Γ ++ [(x, {1 ~r> v2} (mk_op_ret op ^r^ v1))] }) (e ^t^ x) -> *)
+(*     ⅋{st}⟦τ⟧{Γ ++ [(x, {1 ~r> v2} (mk_op_ret op ^r^ v1))] } (tletbiop op v1 v2 e). *)
+(* Proof. *)
+(*   induction Γ; intros; RD_simp2. *)
+(*   - mydestr. inv_rd_simpl1. constructor; auto. *)
+(*     + denotation_simp. assert ([] ⊢t tletbiop op v1 v2 e ⋮t ⌊τ⌋). eapply tletbiop_typable; refinement_solver. *)
+(*       basic_typing_solver. *)
+(*     + exists (eval_op_under_bound_tm op v1 v2). split. apply rR_eval_op_under_bound_tm. *)
+(*       intros. assert (x1 ↪* v_x) as Hz by (eapply rR_eval_op_under_bound_tm_min; eauto). *)
+(*       auto_under v_x. RD_simp2. simpl. *)
+(*       rewrite subst_fresh_tm; auto. rewrite open_subst_same_tm in H10; auto. *)
+(*       eapply termR_perserve_rR; refinement_solver. *)
+(*       eapply letapp_eval_op_under_bound_tm_termR; eauto; refinement_solver. *)
+(*   - constructor; auto. denotation_simp. apply tletbiop_typable_ctx_dummy_cons; auto. *)
+(*     intros. auto_under c_x. simpl. eapply IHΓ; eauto. *)
+(*     + rewrite fv_of_subst_tm_closed; refinement_solver. *)
+(*     + rewrite <- subst_open_var_tm; auto. denotation_simp. basic_typing_solver. *)
+(*   - constructor; auto. denotation_simp. apply tletbiop_typable_ctx_dummy_cons; auto. *)
+(*     mydestr. auto_meet_exists Hmeet. auto_meet_reduce. auto_under v_x. eapply IHΓ; eauto; fold tm_subst. *)
+(*     + rewrite fv_of_subst_tm_closed; refinement_solver. *)
+(*     + rewrite <- subst_open_var_tm; auto. denotation_simp. basic_typing_solver. op_solver1. *)
+(*   - constructor; auto. denotation_simp. apply tletbiop_typable_ctx_dummy_cons; auto. *)
+(*     intros. auto_under v_x. eapply IHΓ; eauto; fold tm_subst. *)
+(*     + rewrite fv_of_subst_tm_closed; refinement_solver. *)
+(*     + rewrite <- subst_open_var_tm; auto. denotation_simp. basic_typing_solver. refinement_solver. *)
+(* Qed. *)
+
+
